首先，我们选择两个数，使得其 gcd 为 `1`

则我们可以把等式变为

`a + b + 1 = n`

进而有

`b = n - 1 - a`

枚举所有可能的 `a` 计算出 `b` 即可

```
typedef long long ll;
#include <bits/stdc++.h>

using namespace std;

#define rep(i, a, b) for (int i = (a); i < (b); i++)
#define all(cont) cont.begin(), cont.end()
#define ms(a) memset(a, 0, sizeof(a))
#define EPS 1e-9
	
template<class T> void chmax(T & a, const T & b) { a = max(a, b); } 
template<class T> void chmin(T & a, const T & b) { a = min(a, b); } 
template <class T> void oa(const vector<T>& a) { for (int i = 0; i < a.size(); ++i) cout << a[i] << " \n"[i + 1 == a.size()]; }
typedef long long ll;
ll mod = 1e9 + 7;

void solve() {
	ll n;
	cin >> n;
	rep (a, 2, n + 1) {
		ll b = n - 1 - a;
		if (__gcd((ll)a, b) == 1 && a != b) {
			cout << a << " " << b << " " << 1 << endl;
			return;
		}
	}
}

	
int main() {
	ios_base::sync_with_stdio(0);
	cin.tie(nullptr);
	
	int q;
	cin >> q;
	while (q--)
		solve();
	
}

// FAST CP: D:\Codes\problem-goods\playground
```